LiveVerif/src/LiveVerifExamples/onesize_malloc.v
@@ -148,8 +148,7 @@ uintptr_t malloc (uintptr_t n) /**#
 Derive malloc SuchThat (fun_correct! malloc) As malloc_ok.                      .**/
 {                                                                          /**. .**/
   uintptr_t l = load(malloc_state_ptr);                                    /**. .**/
-  uintptr_t p = 0;                                                         /**. .**/
-  if (l != 0 && n <= malloc_block_size) {                                  /**.
+  if (l != 0 && n <= malloc_block_size) /* split */ {                      /**.
 
     let H := constr:(#(fixed_size_free_list ?? ??)) in inversion H; clear H.
     (* TODO better inversion tactic for such use cases *)
@@ -160,8 +159,7 @@ Derive malloc SuchThat (fun_correct! malloc) As malloc_ok.                      
            end.
     repeat heapletwise_step.
                                                                                 .**/
-    store(malloc_state_ptr, load(l));                                      /**. .**/
-    p = l;                                                                 /**.
+    store(malloc_state_ptr, load(l));                                      /**.
 
     let H := constr:(#(array (uint 8))) in rename H into h.
     unfold with_mem in h.
@@ -172,10 +170,11 @@ Derive malloc SuchThat (fun_correct! malloc) As malloc_ok.                      
     | ?p ?m => change (with_mem m p) in h
     end.
                                                                                 .**/
-  } else {                                                                 /**. .**/
-    /* empty */                                                            /**. .**/
+    return l;                                                              /**. .**/
   }                                                                        /**. .**/
-  return p;                                                                /**. .**/
+  else {                                                                   /**. .**/
+    return NULL;                                                           /**. .**/
+  }                                                                        /**. .**/
 }                                                                          /**.
 Qed.
 
